src/dvspec/dafny/att_spec_proofs/proof_test.dfy
@@ -22,10 +22,34 @@ module Proof_Test
     import opened Att_Ind_Inv_With_Empty_Initial_Attestation_Slashing_DB
     import opened Helper_Sets_Lemmas
 
+/*
+    lemma test_inv1(dvn: DVState)
+    requires inv1(dvn)
+    ensures && var all_nodes := dvn.all_nodes;
+            && var honest_nodes := dvn.honest_nodes_states.Keys;
+            && var dishonest_nodes := dvn.adversary.nodes;
+            && 2 * |dishonest_nodes| < |honest_nodes|
+    {     
+      var all_nodes := dvn.all_nodes;
+      var honest_nodes := dvn.honest_nodes_states.Keys;
+      var dishonest_nodes := dvn.adversary.nodes;   
+      lemmaQuorumIsGreaterThan2F(all_nodes);
 
+      calc {
+            |honest_nodes|;
+            >= 
+            quorum(|all_nodes|);
+            >
+            { lemmaQuorumIsGreaterThan2F(all_nodes); }
+            2 * f(|all_nodes|);
+            >=
+            2 * |dishonest_nodes|;
+        }
+    }
+*/
 
-    lemma prop52_a(dvn: DVState, hn: BLSPubkey)       
-    requires inv52(dvn)    
+    lemma prop1_a(dvn: DVState, hn: BLSPubkey)       
+    requires inv1(dvn)    
     requires hn in dvn.honest_nodes_states.Keys
     ensures hn in dvn.all_nodes
     ensures hn !in dvn.adversary.nodes
