src/dvspec/dafny/specification/dvn.dfy
@@ -2,6 +2,8 @@ include "../commons.dfy"
 include "dvc_spec.dfy"
 include "consensus.dfy"
 include "network.dfy"
+include "../att_spec_proofs/inv.dfy"
+
 
 module DV 
 {
@@ -11,6 +13,7 @@ module DV
     import opened ConsensusSpec
     import opened DVCNode_Spec
     import opened DVCNode_Externs_Proofs
+    
 
     datatype Adversary = Adversary(
         nodes: set<BLSPubkey>  
@@ -115,6 +118,21 @@ module DV
                 ::
                     s.sequence_attestation_duties_to_be_served[i].attestation_duty.slot <= s.sequence_attestation_duties_to_be_served[j].attestation_duty.slot
         )
+        && ( forall k1: nat, k2: nat :: 
+                s.sequence_attestation_duties_to_be_served[k1].attestation_duty.slot 
+                    == s.sequence_attestation_duties_to_be_served[k2].attestation_duty.slot  
+                ==> 
+                s.sequence_attestation_duties_to_be_served[k1].attestation_duty
+                    == s.sequence_attestation_duties_to_be_served[k2].attestation_duty
+           )
+        && ( forall k1: nat, k2: nat :: 
+                && k1 < k2
+                && s.sequence_attestation_duties_to_be_served[k1].node 
+                    == s.sequence_attestation_duties_to_be_served[k2].node
+                ==> 
+                s.sequence_attestation_duties_to_be_served[k1].attestation_duty.slot 
+                    < s.sequence_attestation_duties_to_be_served[k2].attestation_duty.slot  
+           )
     }
     
     predicate Next(
@@ -135,7 +153,7 @@ module DV
         && dvn.construct_signed_attestation_signature
                 == dvn'.construct_signed_attestation_signature
         && dvn.sequence_attestation_duties_to_be_served
-                == dvn.sequence_attestation_duties_to_be_served
+                == dvn'.sequence_attestation_duties_to_be_served
     }
 
     predicate NextEvent(
